success

src/Init/Data/Range/Polymorphic/SInt.lean
@@ -151,148 +151,6 @@ scoped instance instRxiLawfulHasSize [m : HasModel α β] [Rxi.HasSize β] [Rxi.
     simp only [this, instRxiHasSize]
     apply Rxi.LawfulHasSize.size_eq_succ_of_succ?_eq_some
 
-end HasModel
-
-namespace Int8
-
-open BitVec.Signed
-open scoped HasModel
-
-attribute [-instance] BitVec.instUpwardEnumerable BitVec.instHasSize BitVec.instHasSize_1
-  BitVec.instHasSize_2 BitVec.instLawfulUpwardEnumerable
-
-instance : UpwardEnumerable Int8 where
-  succ? i := if i + 1 = Int8.minValue then none else some (i + 1)
-  succMany? n i :=
-    have := i.minValue_le_toInt
-    if h : i.toInt + n ≤ Int8.maxValue.toInt then some (.ofIntLE _ (by omega) h) else none
-
-instance : HasModel Int8 (BitVec 8) where
-  encode x := x.toBitVec
-  decode x := .ofBitVec x
-  encode_decode := by simp
-  decode_encode := by simp
-  le_iff_encode_le := by simp [Int8.le_iff_toBitVec_sle, BitVec.Signed.instLE]
-  lt_iff_encode_lt := by simp [Int8.lt_iff_toBitVec_slt, BitVec.Signed.instLT]
-
-theorem instUpwardEnumerable_eq :
-    instUpwardEnumerable = HasModel.instUpwardEnumerable := by
-  simp only [instUpwardEnumerable, HasModel.instUpwardEnumerable,
-    HasModel.encode, HasModel.decode, UpwardEnumerable.succ?,
-    UpwardEnumerable.succMany?]
-  congr 1
-  · ext x y
-    simp [← Int8.toBitVec_inj, ← BitVec.eq_sub_iff_add_eq, rotate, BitVec.sub_sub]
-  · ext n x y
-    have h₁ : ∀ n, (2 : Int) ^ n = ↑((2 : Nat) ^ n) := by simp
-    have h₂ : ∀ x : Int8, x - ofNat (2 ^ 7) = x + ofNat (2 ^ 7) := by simp
-    simp [h₁, h₂, ← Int8.toInt_toBitVec, toInt_eq_ofNat_toNat_rotate_sub (show 8 > 0 by omega),
-      rotate, BitVec.ofNatLT_eq_ofNat, ofIntLE_eq_ofInt, Int8.ofInt_eq_ofNat,
-      ofInt_eq_ofNat, Int8.add_assoc, Int8.add_comm (ofNat (2 ^ 7)), and_congr_left_iff,
-      - Int.reducePow, - Nat.reducePow, - Int.natCast_pow, - Int.natCast_add, - Int.natCast_emod, ]
-    omega
-
-instance : LawfulUpwardEnumerable Int8 := by
-  simp only [instUpwardEnumerable_eq]
-  infer_instance
-
-instance : LawfulUpwardEnumerableLE Int8 := by
-  simp only [instUpwardEnumerable_eq]
-  infer_instance
-
-instance : LawfulUpwardEnumerableLT Int8 := inferInstance
-instance : LawfulUpwardEnumerableLT Int8 := inferInstance
-
-instance : Rxc.HasSize Int8 where
-  size lo hi := (hi.toInt + 1 - lo.toInt).toNat
-
-theorem bla {lo hi : BitVec n} (h : n > 0) :
-    (hi.toInt + 1 - lo.toInt).toNat = (rotate hi).toNat + 1 - (rotate lo).toNat := by
-  match n with
-  | 0 => omega
-  | n + 1 =>
-    simp only [toInt_eq_ofNat_toNat_rotate_sub h, rotate, BitVec.toNat_add, Int.natCast_emod,
-      show ∀ a b c d : Int, (a - b) + c - (d - b) = a + c - d by omega]
-    omega
-
-theorem instRxcHasSize_eq :
-    instHasSize = HasModel.instRxcHasSize := by
-  simp only [instHasSize, HasModel.instRxcHasSize, Rxc.HasSize.size, HasModel.encode,
-    ← toInt_toBitVec, bla (Nat.zero_lt_succ _)]
-
-private theorem ofBitVec_eq_iff {x : BitVec 8} {y : Int8} :
-    Int8.ofBitVec x = y ↔ x = y.toBitVec := by
-  rw [← toBitVec_ofBitVec x, toBitVec_inj, toBitVec_ofBitVec]
-
-instance : Rxc.LawfulHasSize Int8 := by
-  simp only [instUpwardEnumerable_eq, instRxcHasSize_eq]
-  infer_instance
-instance : Rxc.IsAlwaysFinite Int8 := inferInstance
-
-instance : Rxo.HasSize Int8 := .ofClosed
-instance : Rxo.LawfulHasSize Int8 := inferInstance
-instance : Rxo.IsAlwaysFinite Int8 := inferInstance
-
-instance instRxiHasSize : Rxi.HasSize Int8 where
-  size lo := ((2 : Int) ^ 7 - lo.toInt).toNat
-
-theorem instRxiHasSize_eq :
-    instRxiHasSize = HasModel.instRxiHasSize := by
-  simp only [instRxiHasSize, HasModel.instRxiHasSize, Rxi.HasSize.size, HasModel.encode,
-    ← toInt_toBitVec, toInt_eq_ofNat_toNat_rotate_sub (Nat.zero_lt_succ _), Int.toNat_sub,
-    show ∀ a : Int, (2 ^ 7) - (a - (2 ^ 7)) = ↑((2 : Nat) ^ 8) - a by omega]
-
-instance : Rxi.LawfulHasSize Int8 := by
-  simp only [instUpwardEnumerable_eq, instRxiHasSize_eq]
-  infer_instance
-instance : Rxi.IsAlwaysFinite Int8 := inferInstance
-
-end Int8
-
-namespace Int16
-
-open BitVec.Signed
-open scoped HasModel
-
-attribute [-instance] BitVec.instUpwardEnumerable BitVec.instHasSize BitVec.instHasSize_1
-  BitVec.instHasSize_2 BitVec.instLawfulUpwardEnumerable
-
-@[inline]
-def irredMin := Int16.minValue
-theorem irredMin_def : irredMin = Int16.minValue := (rfl)
-seal irredMin
-
-@[inline]
-def irredMax := Int16.maxValue
-theorem irredMax_def : irredMax = Int16.maxValue := (rfl)
-seal irredMax
-
-theorem toBitVec_irredMin_eq_irredMin :
-    irredMin.toBitVec = BitVec.Signed.irredMin 16 := by
-  simp [irredMin_def, BitVec.Signed.irredMin_def]
-
-theorem toBitVec_irredMax_eq_irredMax :
-    irredMax.toBitVec = BitVec.Signed.irredMax 16 := by
-  simp [irredMax_def, BitVec.Signed.irredMax_def]
-
-instance : UpwardEnumerable Int16 where
-  succ? i := if i + 1 = irredMin then none else some (i + 1)
-  succMany? n i :=
-    have := i.minValue_le_toInt
-    if h : i.toInt + n ≤ irredMax.toInt then some (.ofIntLE _ (by omega) (irredMax_def ▸ h)) else none
-
-instance : HasModel Int16 (BitVec 16) where
-  encode x := x.toBitVec
-  decode x := .ofBitVec x
-  encode_decode := by simp
-  decode_encode := by simp
-  le_iff_encode_le := by simp [Int16.le_iff_toBitVec_sle, BitVec.Signed.instLE]
-  lt_iff_encode_lt := by simp [Int16.lt_iff_toBitVec_slt, BitVec.Signed.instLT]
-
-private theorem ofBitVec_eq_iff {x : BitVec 16} {y : Int16} :
-    Int16.ofBitVec x = y ↔ x = y.toBitVec := by
-  rw [← toBitVec_ofBitVec x, toBitVec_inj, toBitVec_ofBitVec]
-
 theorem general_succ? {α : Type u} [UpwardEnumerable α] [LE α] [LT α] [m : HasModel α (BitVec n)]
     {x : α}
     (h : ∀ y, succ? x = some y ↔ ¬ m.encode x + 1#n = BitVec.Signed.irredMin n ∧ m.encode x + 1#n = m.encode y) :
@@ -318,32 +176,128 @@ theorem general_succMany? {α : Type u} [UpwardEnumerable α] [LE α] [LT α] [m
     simp only [ofNat_eq_rotate_ofInt_sub, rotate_rotate]
     congr; omega
 
-theorem instUpwardEnumerable_eq :
-    instUpwardEnumerable = HasModel.instUpwardEnumerable := by
-  apply UpwardEnumerable.ext
-  · apply funext; intro x
-    apply general_succ?
-    intro y
-    simp [HasModel.encode, succ?, ← Int16.toBitVec_inj, toBitVec_irredMin_eq_irredMin]
-  · apply funext; intro n; apply funext; intro x
-    simp [general_succMany?, instUpwardEnumerable, HasModel.encode, HasModel.decode,
-      ← toInt_toBitVec, toBitVec_irredMax_eq_irredMax, ofIntLE_eq_ofInt]
+theorem general_rxcSize {lo hi : BitVec n} (h : n > 0) :
+    (hi.toInt + 1 - lo.toInt).toNat = (rotate hi).toNat + 1 - (rotate lo).toNat := by
+  match n with
+  | 0 => omega
+  | n + 1 =>
+    simp only [toInt_eq_ofNat_toNat_rotate_sub h, rotate, BitVec.toNat_add, Int.natCast_emod,
+      show ∀ a b c d : Int, (a - b) + c - (d - b) = a + c - d by omega]
+    omega
+
+theorem general_rxiSize {lo : BitVec n} (h : n > 0) :
+    (2 ^ (n - 1) - lo.toInt).toNat = 2 ^ n - (rotate lo).toNat := by
+  simp only [toInt_eq_ofNat_toNat_rotate_sub h]
+  simp only [Int.sub_eq_add_neg, Int.neg_add, Int.neg_neg, Int.add_comm _ (2 ^ (n - 1)),
+    ← Int.add_assoc,
+    show (2 : Int) ^ (n - 1) + 2 ^ (n - 1) = 2 ^ (n - 1 + 1) by omega,
+    show n - 1 + 1 = n by omega]
+  simp [← Int.sub_eq_add_neg, Int.toNat_sub', Int.toNat_pow_of_nonneg]
+
+end HasModel
+
+namespace Int8
 
 open BitVec.Signed
 open scoped HasModel
 
-attribute [-instance] BitVec.instUpwardEnumerable BitVec.instHasSize BitVec.instHasSize_1
-  BitVec.instHasSize_2 BitVec.instLawfulUpwardEnumerable
+@[inline] def irredMin := Int8.minValue
+@[inline] def irredMax := Int8.maxValue
+theorem irredMin_def : irredMin = Int8.minValue := (rfl)
+theorem irredMax_def : irredMax = Int8.maxValue := (rfl)
+seal irredMin irredMax
 
-@[inline]
-def irredMin := Int16.minValue
+theorem toBitVec_irredMin_eq_irredMin : irredMin.toBitVec = BitVec.Signed.irredMin 8 := by
+  simp [irredMin_def, BitVec.Signed.irredMin_def]
+theorem toBitVec_irredMax_eq_irredMax : irredMax.toBitVec = BitVec.Signed.irredMax 8 := by
+  simp [irredMax_def, BitVec.Signed.irredMax_def]
+
+instance : UpwardEnumerable Int8 where
+  succ? i := if i + 1 = irredMin then none else some (i + 1)
+  succMany? n i :=
+    have := i.minValue_le_toInt
+    if h : i.toInt + n ≤ irredMax.toInt then some (.ofIntLE _ (by omega) (irredMax_def ▸ h)) else none
+
+instance : HasModel Int8 (BitVec 8) where
+  encode x := x.toBitVec
+  decode x := .ofBitVec x
+  encode_decode := by simp
+  decode_encode := by simp
+  le_iff_encode_le := by simp [Int8.le_iff_toBitVec_sle, BitVec.Signed.instLE]
+  lt_iff_encode_lt := by simp [Int8.lt_iff_toBitVec_slt, BitVec.Signed.instLT]
+
+private theorem ofBitVec_eq_iff {x : BitVec 8} {y : Int8} :
+    Int8.ofBitVec x = y ↔ x = y.toBitVec := by
+  rw [← toBitVec_ofBitVec x, toBitVec_inj, toBitVec_ofBitVec]
+
+theorem instUpwardEnumerable_eq :
+    instUpwardEnumerable = HasModel.instUpwardEnumerable := by
+  apply UpwardEnumerable.ext
+  · apply funext; intro x
+    apply HasModel.general_succ?
+    simp [HasModel.encode, succ?, ← Int8.toBitVec_inj, toBitVec_irredMin_eq_irredMin]
+  · ext
+    simp [HasModel.general_succMany?, instUpwardEnumerable, HasModel.encode, HasModel.decode,
+      ← toInt_toBitVec, toBitVec_irredMax_eq_irredMax, ofIntLE_eq_ofInt]
+
+instance : LawfulUpwardEnumerable Int8 := by
+  simp only [instUpwardEnumerable_eq]
+  infer_instance
+
+instance : LawfulUpwardEnumerableLE Int8 := by
+  simp only [instUpwardEnumerable_eq]
+  infer_instance
+
+instance : LawfulUpwardEnumerableLT Int8 := inferInstance
+instance : LawfulUpwardEnumerableLT Int8 := inferInstance
+
+instance : Rxc.HasSize Int8 where
+  size lo hi := (hi.toInt + 1 - lo.toInt).toNat
+
+theorem instRxcHasSize_eq :
+    instHasSize = HasModel.instRxcHasSize := by
+  simp only [instHasSize, HasModel.instRxcHasSize, Rxc.HasSize.size, HasModel.encode,
+    ← toInt_toBitVec, HasModel.general_rxcSize (Nat.zero_lt_succ _)]
+
+instance : Rxc.LawfulHasSize Int8 := by
+  simp only [instUpwardEnumerable_eq, instRxcHasSize_eq]
+  infer_instance
+instance : Rxc.IsAlwaysFinite Int8 := inferInstance
+
+instance : Rxo.HasSize Int8 := .ofClosed
+instance : Rxo.LawfulHasSize Int8 := inferInstance
+instance : Rxo.IsAlwaysFinite Int8 := inferInstance
+
+instance instRxiHasSize : Rxi.HasSize Int8 where
+  size lo := ((2 : Int) ^ 7 - lo.toInt).toNat
+
+theorem instRxiHasSize_eq :
+    instRxiHasSize = HasModel.instRxiHasSize := by
+  simp only [instRxiHasSize, HasModel.instRxiHasSize, Rxi.HasSize.size, ← toInt_toBitVec,
+    HasModel.encode, HasModel.general_rxiSize (show 8 > 0 by omega)]
+
+instance : Rxi.LawfulHasSize Int8 := by
+  simp only [instUpwardEnumerable_eq, instRxiHasSize_eq]
+  infer_instance
+instance : Rxi.IsAlwaysFinite Int8 := inferInstance
+
+end Int8
+
+namespace Int16
+
+open BitVec.Signed
+open scoped HasModel
+
+@[inline] def irredMin := Int16.minValue
+@[inline] def irredMax := Int16.maxValue
 theorem irredMin_def : irredMin = Int16.minValue := (rfl)
-seal irredMin
-
-@[inline]
-def irredMax := Int16.maxValue
 theorem irredMax_def : irredMax = Int16.maxValue := (rfl)
-seal irredMax
+seal irredMin irredMax
+
+theorem toBitVec_irredMin_eq_irredMin : irredMin.toBitVec = BitVec.Signed.irredMin 16 := by
+  simp [irredMin_def, BitVec.Signed.irredMin_def]
+theorem toBitVec_irredMax_eq_irredMax : irredMax.toBitVec = BitVec.Signed.irredMax 16 := by
+  simp [irredMax_def, BitVec.Signed.irredMax_def]
 
 instance : UpwardEnumerable Int16 where
   succ? i := if i + 1 = irredMin then none else some (i + 1)
@@ -359,82 +313,19 @@ instance : HasModel Int16 (BitVec 16) where
   le_iff_encode_le := by simp [Int16.le_iff_toBitVec_sle, BitVec.Signed.instLE]
   lt_iff_encode_lt := by simp [Int16.lt_iff_toBitVec_slt, BitVec.Signed.instLT]
 
--- theorem bla {x : Int16} :
---     (succ? x) = (if (x.toBitVec + 1 = - 2 ^ 15) then none else some (x.toBitVec + 1)).map .ofBitVec := by
---   sorry
-
--- #print instUpwardEnumerable
-
--- axiom sry {α} : α
-
--- seal HasModel.instUpwardEnumerable
-
--- theorem ex :
---     sry = (HasModel.instUpwardEnumerable : UpwardEnumerable Int16) := by
---   apply UpwardEnumerable.ext
---   · apply funext; intro x
---     generalize h : @succ? Int16 sry x = g
---     rw [bla] at h
---     rw [bla]
-
-theorem bla {x : Int16} :
-    (succ? x) = (if (x.toBitVec + 1 = - 2 ^ 15) then none else some (x.toBitVec + 1)).map .ofBitVec := by
-  simp only [← BitVec.eq_sub_iff_add_eq, succ?, ← toBitVec_inj,
-    show minValue.toBitVec = - 2 ^ 15 by rfl, Int16.toBitVec_add, toBitVec_ofNat]
-  split <;> simp
-
-#print instUpwardEnumerable
-
---seal HasModel.instUpwardEnumerable
---seal instUpwardEnumerable
-
-theorem ex :
-    instUpwardEnumerable = HasModel.instUpwardEnumerable := by
-  apply UpwardEnumerable.ext
-  · apply funext; intro x
-    refine Eq.trans bla ?_
-
-
-  simp only [instUpwardEnumerable, HasModel.instUpwardEnumerable, HasModel.encode,
-    HasModel.decode]
-  -- simp only [instUpwardEnumerable, HasModel.instUpwardEnumerable,
-  --   HasModel.encode, HasModel.decode, UpwardEnumerable.succ?,
-  --   UpwardEnumerable.succMany?]
-  -- have : ∀ {s sm s' sm'}, sm = sm' → UpwardEnumerable.mk s sm = (UpwardEnumerable.mk s' sm' : UpwardEnumerable Int16) := by
-  --   sorry
-
-  -- apply this
-  -- · ext n x y
-  --   simp only [← toInt_toBitVec, toInt_eq_ofNat_toNat_rotate_sub (show 16 > 0 by omega), rotate,
-  --     BitVec.natCast_eq_ofNat, BitVec.toNat_add, BitVec.toNat_ofNat]
-  --   simp only [ofIntLE_eq_ofInt]
-  --   -- simp [h₁, h₂, ← Int16.toInt_toBitVec, toInt_eq_ofNat_toNat_rotate_sub (show 16 > 0 by omega),
-  --   --   rotate, BitVec.ofNatLT_eq_ofNat, ofIntLE_eq_ofInt, Int16.ofInt_eq_ofNat,
-  --   --   ofInt_eq_ofNat, Int16.add_assoc, Int16.add_comm (ofNat (2 ^ 15)), and_congr_left_iff,
-  --   --   - Int.reducePow, - Nat.reducePow, - Int.natCast_pow, - Int.natCast_add, - Int.natCast_emod, ]
-  --   omega
+private theorem ofBitVec_eq_iff {x : BitVec 16} {y : Int16} :
+    Int16.ofBitVec x = y ↔ x = y.toBitVec := by
+  rw [← toBitVec_ofBitVec x, toBitVec_inj, toBitVec_ofBitVec]
 
 theorem instUpwardEnumerable_eq :
     instUpwardEnumerable = HasModel.instUpwardEnumerable := by
-  simp only [instUpwardEnumerable, HasModel.instUpwardEnumerable,
-    HasModel.encode, HasModel.decode, UpwardEnumerable.succ?,
-    UpwardEnumerable.succMany?]
-  have : ∀ {s sm s' sm'}, s = s' → sm = sm' → UpwardEnumerable.mk s sm = (UpwardEnumerable.mk s' sm' : UpwardEnumerable Int16) := by
-    sorry
-  apply this
-  --congr 1
-  · sorry
-    -- ext x y
-    -- simp [← Int16.toBitVec_inj, ← BitVec.eq_sub_iff_add_eq, rotate, BitVec.sub_sub]
-  · ext n x y
-    simp only [← toInt_toBitVec, toInt_eq_ofNat_toNat_rotate_sub (show 16 > 0 by omega), rotate,
-      BitVec.natCast_eq_ofNat, BitVec.toNat_add, BitVec.toNat_ofNat]
-    simp only [ofIntLE_eq_ofInt]
-    -- simp [h₁, h₂, ← Int16.toInt_toBitVec, toInt_eq_ofNat_toNat_rotate_sub (show 16 > 0 by omega),
-    --   rotate, BitVec.ofNatLT_eq_ofNat, ofIntLE_eq_ofInt, Int16.ofInt_eq_ofNat,
-    --   ofInt_eq_ofNat, Int16.add_assoc, Int16.add_comm (ofNat (2 ^ 15)), and_congr_left_iff,
-    --   - Int.reducePow, - Nat.reducePow, - Int.natCast_pow, - Int.natCast_add, - Int.natCast_emod, ]
-    omega
+  apply UpwardEnumerable.ext
+  · apply funext; intro x
+    apply HasModel.general_succ?
+    simp [HasModel.encode, succ?, ← Int16.toBitVec_inj, toBitVec_irredMin_eq_irredMin]
+  · ext
+    simp [HasModel.general_succMany?, instUpwardEnumerable, HasModel.encode, HasModel.decode,
+      ← toInt_toBitVec, toBitVec_irredMax_eq_irredMax, ofIntLE_eq_ofInt]
 
 instance : LawfulUpwardEnumerable Int16 := by
   simp only [instUpwardEnumerable_eq]
@@ -450,23 +341,10 @@ instance : LawfulUpwardEnumerableLT Int16 := inferInstance
 instance : Rxc.HasSize Int16 where
   size lo hi := (hi.toInt + 1 - lo.toInt).toNat
 
-theorem bla {lo hi : BitVec n} (h : n > 0) :
-    (hi.toInt + 1 - lo.toInt).toNat = (rotate hi).toNat + 1 - (rotate lo).toNat := by
-  match n with
-  | 0 => omega
-  | n + 1 =>
-    simp only [toInt_eq_ofNat_toNat_rotate_sub h, rotate, BitVec.toNat_add, Int.natCast_emod,
-      show ∀ a b c d : Int, (a - b) + c - (d - b) = a + c - d by omega]
-    omega
-
 theorem instRxcHasSize_eq :
     instHasSize = HasModel.instRxcHasSize := by
   simp only [instHasSize, HasModel.instRxcHasSize, Rxc.HasSize.size, HasModel.encode,
-    ← toInt_toBitVec, bla (Nat.zero_lt_succ _)]
-
-private theorem ofBitVec_eq_iff {x : BitVec 16} {y : Int16} :
-    Int16.ofBitVec x = y ↔ x = y.toBitVec := by
-  rw [← toBitVec_ofBitVec x, toBitVec_inj, toBitVec_ofBitVec]
+    ← toInt_toBitVec, HasModel.general_rxcSize (Nat.zero_lt_succ _)]
 
 instance : Rxc.LawfulHasSize Int16 := by
   simp only [instUpwardEnumerable_eq, instRxcHasSize_eq]
@@ -482,9 +360,8 @@ instance instRxiHasSize : Rxi.HasSize Int16 where
 
 theorem instRxiHasSize_eq :
     instRxiHasSize = HasModel.instRxiHasSize := by
-  simp only [instRxiHasSize, HasModel.instRxiHasSize, Rxi.HasSize.size, HasModel.encode,
-    ← toInt_toBitVec, toInt_eq_ofNat_toNat_rotate_sub (Nat.zero_lt_succ _), Int.toNat_sub,
-    show ∀ a : Int, (2 ^ 15) - (a - (2 ^ 15)) = ↑((2 : Nat) ^ 16) - a by omega]
+  simp only [instRxiHasSize, HasModel.instRxiHasSize, Rxi.HasSize.size, ← toInt_toBitVec,
+    HasModel.encode, HasModel.general_rxiSize (show 16 > 0 by omega)]
 
 instance : Rxi.LawfulHasSize Int16 := by
   simp only [instUpwardEnumerable_eq, instRxiHasSize_eq]
@@ -493,495 +370,57 @@ instance : Rxi.IsAlwaysFinite Int16 := inferInstance
 
 end Int16
 
-namespace Int8
-
-open BitVec.Signed
-open scoped HasModel
-
-attribute [-instance] BitVec.instUpwardEnumerable BitVec.instHasSize BitVec.instHasSize_1
-  BitVec.instHasSize_2 BitVec.instLawfulUpwardEnumerable
-
-instance : UpwardEnumerable Int8 where
-  succ? i := if i + 1 = Int8.minValue then none else some (i + 1)
-  succMany? n i :=
-    have := i.minValue_le_toInt
-    if h : i.toInt + n ≤ Int8.maxValue.toInt then some (.ofIntLE _ (by omega) h) else none
-
-instance : HasModel Int8 (BitVec 8) where
-  encode x := x.toBitVec
-  decode x := .ofBitVec x
-  encode_decode := by simp
-  decode_encode := by simp
-  le_iff_encode_le := by simp [Int8.le_iff_toBitVec_sle, BitVec.Signed.instLE]
-  lt_iff_encode_lt := by simp [Int8.lt_iff_toBitVec_slt, BitVec.Signed.instLT]
-
-theorem instUpwardEnumerable_eq :
-    instUpwardEnumerable = HasModel.instUpwardEnumerable := by
-  simp only [instUpwardEnumerable, HasModel.instUpwardEnumerable,
-    HasModel.encode, HasModel.decode, UpwardEnumerable.succ?,
-    UpwardEnumerable.succMany?]
-  congr 1
-  · ext x y
-    simp [← Int8.toBitVec_inj, ← BitVec.eq_sub_iff_add_eq, rotate, BitVec.sub_sub]
-  · ext n x y
-    have h₁ : ∀ n, (2 : Int) ^ n = ↑((2 : Nat) ^ n) := by simp
-    have h₂ : ∀ x : Int8, x - ofNat (2 ^ 7) = x + ofNat (2 ^ 7) := by simp
-    simp [h₁, h₂, ← Int8.toInt_toBitVec, toInt_eq_ofNat_toNat_rotate_sub (show 8 > 0 by omega),
-      rotate, BitVec.ofNatLT_eq_ofNat, ofIntLE_eq_ofInt, Int8.ofInt_eq_ofNat,
-      ofInt_eq_ofNat, Int8.add_assoc, Int8.add_comm (ofNat (2 ^ 7)), and_congr_left_iff,
-      - Int.reducePow, - Nat.reducePow, - Int.natCast_pow, - Int.natCast_add, - Int.natCast_emod, ]
-    omega
-
-instance : LawfulUpwardEnumerable Int8 := by
-  simp only [instUpwardEnumerable_eq]
-  infer_instance
-
-instance : LawfulUpwardEnumerableLE Int8 := by
-  simp only [instUpwardEnumerable_eq]
-  infer_instance
-
-instance : LawfulUpwardEnumerableLT Int8 := inferInstance
-instance : LawfulUpwardEnumerableLT Int8 := inferInstance
-
-instance : Rxc.HasSize Int8 where
-  size lo hi := (hi.toInt + 1 - lo.toInt).toNat
-
-theorem bla {lo hi : BitVec n} (h : n > 0) :
-    (hi.toInt + 1 - lo.toInt).toNat = (rotate hi).toNat + 1 - (rotate lo).toNat := by
-  match n with
-  | 0 => omega
-  | n + 1 =>
-    simp only [toInt_eq_ofNat_toNat_rotate_sub h, rotate, BitVec.toNat_add, Int.natCast_emod,
-      show ∀ a b c d : Int, (a - b) + c - (d - b) = a + c - d by omega]
-    omega
-
-theorem instRxcHasSize_eq :
-    instHasSize = HasModel.instRxcHasSize := by
-  simp only [instHasSize, HasModel.instRxcHasSize, Rxc.HasSize.size, HasModel.encode,
-    ← toInt_toBitVec, bla (Nat.zero_lt_succ _)]
-
-private theorem ofBitVec_eq_iff {x : BitVec 8} {y : Int8} :
-    Int8.ofBitVec x = y ↔ x = y.toBitVec := by
-  rw [← toBitVec_ofBitVec x, toBitVec_inj, toBitVec_ofBitVec]
-
-instance : Rxc.LawfulHasSize Int8 := by
-  simp only [instUpwardEnumerable_eq, instRxcHasSize_eq]
-  infer_instance
-instance : Rxc.IsAlwaysFinite Int8 := inferInstance
-
-instance : Rxo.HasSize Int8 := .ofClosed
-instance : Rxo.LawfulHasSize Int8 := inferInstance
-instance : Rxo.IsAlwaysFinite Int8 := inferInstance
-
-instance instRxiHasSize : Rxi.HasSize Int8 where
-  size lo := ((2 : Int) ^ 7 - lo.toInt).toNat
-
-theorem instRxiHasSize_eq :
-    instRxiHasSize = HasModel.instRxiHasSize := by
-  simp only [instRxiHasSize, HasModel.instRxiHasSize, Rxi.HasSize.size, HasModel.encode,
-    ← toInt_toBitVec, toInt_eq_ofNat_toNat_rotate_sub (Nat.zero_lt_succ _), Int.toNat_sub,
-    show ∀ a : Int, (2 ^ 7) - (a - (2 ^ 7)) = ↑((2 : Nat) ^ 8) - a by omega]
-
-instance : Rxi.LawfulHasSize Int8 := by
-  simp only [instUpwardEnumerable_eq, instRxiHasSize_eq]
-  infer_instance
-instance : Rxi.IsAlwaysFinite Int8 := inferInstance
-
-end Int8
-
-namespace Int8
-
-open BitVec.Signed
-open scoped HasModel
-
-attribute [-instance] BitVec.instUpwardEnumerable BitVec.instHasSize BitVec.instHasSize_1
-  BitVec.instHasSize_2 BitVec.instLawfulUpwardEnumerable
-
-instance : UpwardEnumerable Int8 where
-  succ? i := if i + 1 = Int8.minValue then none else some (i + 1)
-  succMany? n i :=
-    have := i.minValue_le_toInt
-    if h : i.toInt + n ≤ Int8.maxValue.toInt then some (.ofIntLE _ (by omega) h) else none
-
-instance : HasModel Int8 (BitVec 8) where
-  encode x := x.toBitVec
-  decode x := .ofBitVec x
-  encode_decode := by simp
-  decode_encode := by simp
-  le_iff_encode_le := by simp [Int8.le_iff_toBitVec_sle, BitVec.Signed.instLE]
-  lt_iff_encode_lt := by simp [Int8.lt_iff_toBitVec_slt, BitVec.Signed.instLT]
-
-theorem instUpwardEnumerable_eq :
-    instUpwardEnumerable = HasModel.instUpwardEnumerable := by
-  simp only [instUpwardEnumerable, HasModel.instUpwardEnumerable,
-    HasModel.encode, HasModel.decode, UpwardEnumerable.succ?,
-    UpwardEnumerable.succMany?]
-  congr 1
-  · ext x y
-    simp [← Int8.toBitVec_inj, ← BitVec.eq_sub_iff_add_eq, rotate, BitVec.sub_sub]
-  · ext n x y
-    have h₁ : ∀ n, (2 : Int) ^ n = ↑((2 : Nat) ^ n) := by simp
-    have h₂ : ∀ x : Int8, x - ofNat (2 ^ 7) = x + ofNat (2 ^ 7) := by simp
-    simp [h₁, h₂, ← Int8.toInt_toBitVec, toInt_eq_ofNat_toNat_rotate_sub (show 8 > 0 by omega),
-      rotate, BitVec.ofNatLT_eq_ofNat, ofIntLE_eq_ofInt, Int8.ofInt_eq_ofNat,
-      ofInt_eq_ofNat, Int8.add_assoc, Int8.add_comm (ofNat (2 ^ 7)), and_congr_left_iff,
-      - Int.reducePow, - Nat.reducePow, - Int.natCast_pow, - Int.natCast_add, - Int.natCast_emod, ]
-    omega
-
-instance : LawfulUpwardEnumerable Int8 := by
-  simp only [instUpwardEnumerable_eq]
-  infer_instance
-
-instance : LawfulUpwardEnumerableLE Int8 := by
-  simp only [instUpwardEnumerable_eq]
-  infer_instance
-
-instance : LawfulUpwardEnumerableLT Int8 := inferInstance
-instance : LawfulUpwardEnumerableLT Int8 := inferInstance
-
-instance : Rxc.HasSize Int8 where
-  size lo hi := (hi.toInt + 1 - lo.toInt).toNat
-
-theorem bla {lo hi : BitVec n} (h : n > 0) :
-    (hi.toInt + 1 - lo.toInt).toNat = (rotate hi).toNat + 1 - (rotate lo).toNat := by
-  match n with
-  | 0 => omega
-  | n + 1 =>
-    simp only [toInt_eq_ofNat_toNat_rotate_sub h, rotate, BitVec.toNat_add, Int.natCast_emod,
-      show ∀ a b c d : Int, (a - b) + c - (d - b) = a + c - d by omega]
-    omega
-
-theorem instRxcHasSize_eq :
-    instHasSize = HasModel.instRxcHasSize := by
-  simp only [instHasSize, HasModel.instRxcHasSize, Rxc.HasSize.size, HasModel.encode,
-    ← toInt_toBitVec, bla (Nat.zero_lt_succ _)]
-
-private theorem ofBitVec_eq_iff {x : BitVec 8} {y : Int8} :
-    Int8.ofBitVec x = y ↔ x = y.toBitVec := by
-  rw [← toBitVec_ofBitVec x, toBitVec_inj, toBitVec_ofBitVec]
-
-instance : Rxc.LawfulHasSize Int8 := by
-  simp only [instUpwardEnumerable_eq, instRxcHasSize_eq]
-  infer_instance
-instance : Rxc.IsAlwaysFinite Int8 := inferInstance
-
-instance : Rxo.HasSize Int8 := .ofClosed
-instance : Rxo.LawfulHasSize Int8 := inferInstance
-instance : Rxo.IsAlwaysFinite Int8 := inferInstance
-
-instance instRxiHasSize : Rxi.HasSize Int8 where
-  size lo := ((2 : Int) ^ 7 - lo.toInt).toNat
-
-theorem instRxiHasSize_eq :
-    instRxiHasSize = HasModel.instRxiHasSize := by
-  simp only [instRxiHasSize, HasModel.instRxiHasSize, Rxi.HasSize.size, HasModel.encode,
-    ← toInt_toBitVec, toInt_eq_ofNat_toNat_rotate_sub (Nat.zero_lt_succ _), Int.toNat_sub,
-    show ∀ a : Int, (2 ^ 7) - (a - (2 ^ 7)) = ↑((2 : Nat) ^ 8) - a by omega]
-
-instance : Rxi.LawfulHasSize Int8 := by
-  simp only [instUpwardEnumerable_eq, instRxiHasSize_eq]
-  infer_instance
-instance : Rxi.IsAlwaysFinite Int8 := inferInstance
-
-end Int8
-
-namespace Int8
-
-open BitVec.Signed
-open scoped HasModel
-
-attribute [-instance] BitVec.instUpwardEnumerable BitVec.instHasSize BitVec.instHasSize_1
-  BitVec.instHasSize_2 BitVec.instLawfulUpwardEnumerable
-
-instance : UpwardEnumerable Int8 where
-  succ? i := if i + 1 = Int8.minValue then none else some (i + 1)
-  succMany? n i :=
-    have := i.minValue_le_toInt
-    if h : i.toInt + n ≤ Int8.maxValue.toInt then some (.ofIntLE _ (by omega) h) else none
-
-instance : HasModel Int8 (BitVec 8) where
-  encode x := x.toBitVec
-  decode x := .ofBitVec x
-  encode_decode := by simp
-  decode_encode := by simp
-  le_iff_encode_le := by simp [Int8.le_iff_toBitVec_sle, BitVec.Signed.instLE]
-  lt_iff_encode_lt := by simp [Int8.lt_iff_toBitVec_slt, BitVec.Signed.instLT]
-
-theorem instUpwardEnumerable_eq :
-    instUpwardEnumerable = HasModel.instUpwardEnumerable := by
-  simp only [instUpwardEnumerable, HasModel.instUpwardEnumerable,
-    HasModel.encode, HasModel.decode, UpwardEnumerable.succ?,
-    UpwardEnumerable.succMany?]
-  congr 1
-  · ext x y
-    simp [← Int8.toBitVec_inj, ← BitVec.eq_sub_iff_add_eq, rotate, BitVec.sub_sub]
-  · ext n x y
-    have h₁ : ∀ n, (2 : Int) ^ n = ↑((2 : Nat) ^ n) := by simp
-    have h₂ : ∀ x : Int8, x - ofNat (2 ^ 7) = x + ofNat (2 ^ 7) := by simp
-    simp [h₁, h₂, ← Int8.toInt_toBitVec, toInt_eq_ofNat_toNat_rotate_sub (show 8 > 0 by omega),
-      rotate, BitVec.ofNatLT_eq_ofNat, ofIntLE_eq_ofInt, Int8.ofInt_eq_ofNat,
-      ofInt_eq_ofNat, Int8.add_assoc, Int8.add_comm (ofNat (2 ^ 7)), and_congr_left_iff,
-      - Int.reducePow, - Nat.reducePow, - Int.natCast_pow, - Int.natCast_add, - Int.natCast_emod, ]
-    omega
-
-instance : LawfulUpwardEnumerable Int8 := by
-  simp only [instUpwardEnumerable_eq]
-  infer_instance
-
-instance : LawfulUpwardEnumerableLE Int8 := by
-  simp only [instUpwardEnumerable_eq]
-  infer_instance
-
-instance : LawfulUpwardEnumerableLT Int8 := inferInstance
-instance : LawfulUpwardEnumerableLT Int8 := inferInstance
-
-instance : Rxc.HasSize Int8 where
-  size lo hi := (hi.toInt + 1 - lo.toInt).toNat
-
-theorem bla {lo hi : BitVec n} (h : n > 0) :
-    (hi.toInt + 1 - lo.toInt).toNat = (rotate hi).toNat + 1 - (rotate lo).toNat := by
-  match n with
-  | 0 => omega
-  | n + 1 =>
-    simp only [toInt_eq_ofNat_toNat_rotate_sub h, rotate, BitVec.toNat_add, Int.natCast_emod,
-      show ∀ a b c d : Int, (a - b) + c - (d - b) = a + c - d by omega]
-    omega
-
-theorem instRxcHasSize_eq :
-    instHasSize = HasModel.instRxcHasSize := by
-  simp only [instHasSize, HasModel.instRxcHasSize, Rxc.HasSize.size, HasModel.encode,
-    ← toInt_toBitVec, bla (Nat.zero_lt_succ _)]
-
-private theorem ofBitVec_eq_iff {x : BitVec 8} {y : Int8} :
-    Int8.ofBitVec x = y ↔ x = y.toBitVec := by
-  rw [← toBitVec_ofBitVec x, toBitVec_inj, toBitVec_ofBitVec]
-
-instance : Rxc.LawfulHasSize Int8 := by
-  simp only [instUpwardEnumerable_eq, instRxcHasSize_eq]
-  infer_instance
-instance : Rxc.IsAlwaysFinite Int8 := inferInstance
-
-instance : Rxo.HasSize Int8 := .ofClosed
-instance : Rxo.LawfulHasSize Int8 := inferInstance
-instance : Rxo.IsAlwaysFinite Int8 := inferInstance
-
-instance instRxiHasSize : Rxi.HasSize Int8 where
-  size lo := ((2 : Int) ^ 7 - lo.toInt).toNat
-
-theorem instRxiHasSize_eq :
-    instRxiHasSize = HasModel.instRxiHasSize := by
-  simp only [instRxiHasSize, HasModel.instRxiHasSize, Rxi.HasSize.size, HasModel.encode,
-    ← toInt_toBitVec, toInt_eq_ofNat_toNat_rotate_sub (Nat.zero_lt_succ _), Int.toNat_sub,
-    show ∀ a : Int, (2 ^ 7) - (a - (2 ^ 7)) = ↑((2 : Nat) ^ 8) - a by omega]
-
-instance : Rxi.LawfulHasSize Int8 := by
-  simp only [instUpwardEnumerable_eq, instRxiHasSize_eq]
-  infer_instance
-instance : Rxi.IsAlwaysFinite Int8 := inferInstance
-
-end Int8
-
-namespace Int16
-
-open BitVec.Signed
-
-attribute [-instance] BitVec.instUpwardEnumerable BitVec.instHasSize BitVec.instHasSize_1
-  BitVec.instHasSize_2 BitVec.instLawfulUpwardEnumerable
-
-instance : UpwardEnumerable Int16 where
-  succ? i := if i + 1 = Int16.minValue then none else some (i + 1)
-  succMany? n i :=
-    have := i.minValue_le_toInt
-    if h : i.toInt + n ≤ Int16.maxValue.toInt then some (.ofIntLE _ (by omega) h) else none
-
-theorem succ?_ofBitVec {x : BitVec 16} :
-    UpwardEnumerable.succ? (Int16.ofBitVec x) = Int16.ofBitVec <$> UpwardEnumerable.succ? x := by
-  simp only [succ?, ← toBitVec_inj, Int16.toBitVec_add, toBitVec_ofBitVec, toBitVec_ofNat,
-    BitVec.ofNat_eq_ofNat, toBitVec_neg, BitVec.reduceNeg, rotate, BitVec.natCast_eq_ofNat,
-    Option.map_eq_map, Option.map_map, Function.comp_def]
-  split <;> split <;> try (simp_all [Int16.add_assoc]; done)
-  all_goals
-    rename_i h h'
-    rw [BitVec.add_assoc, BitVec.add_comm 32768#16 1#16, ← BitVec.add_assoc,
-      ← BitVec.eq_sub_iff_add_eq] at h'
-    simp [h] at h'
-
-theorem succMany?_ofBitVec {k : Nat} {x : BitVec 16} :
-    UpwardEnumerable.succMany? k (Int16.ofBitVec x) =
-      Int16.ofBitVec <$> UpwardEnumerable.succMany? k x := by
-  simp only [succMany?, maxValue, ofIntLE_eq_ofInt, ofInt_add, dite_eq_ite, rotate,
-    BitVec.ofNatLT_eq_ofNat, Option.map_eq_map, Option.map_if, ofBitVec_add, ofBitVec_ofNat,
-    ofNat_add, ofNat_bitVecToNat]
-  split <;> split <;> try (simp [← ofBitVec_ofInt, Int16.add_assoc, Int16.add_comm (-32768)]; done)
-  all_goals
-    rename_i h h'
-    simp [toInt_eq_ofNat_toNat_rotate_sub, rotate] at h h'
-    omega
-
-theorem upwardEnumerableLE_ofBitVec {x y : BitVec 16} :
-    UpwardEnumerable.LE (Int16.ofBitVec x) (Int16.ofBitVec y) ↔ UpwardEnumerable.LE x y := by
-  simp [UpwardEnumerable.LE, succMany?_ofBitVec, ofBitVec_inj]
-
-theorem upwardEnumerableLT_ofBitVec {x y : BitVec 16} :
-    UpwardEnumerable.LT (Int16.ofBitVec x) (Int16.ofBitVec y) ↔ UpwardEnumerable.LT x y := by
-  simp [UpwardEnumerable.LT, succMany?_ofBitVec, ofBitVec_inj]
-
-instance : LawfulUpwardEnumerable Int16 where
-  ne_of_lt x y := by
-    rw [← ofBitVec_toBitVec x, ← ofBitVec_toBitVec y]
-    simpa [upwardEnumerableLT_ofBitVec, ne_iff_ofBitVec_ne, -ofBitVec_toBitVec] using
-      LawfulUpwardEnumerable.ne_of_lt (α := BitVec 16) _ _
-  succMany?_zero x := by
-    rw [← ofBitVec_toBitVec x]
-    simpa [succMany?_ofBitVec, ofBitVec_inj, -ofBitVec_toBitVec] using succMany?_zero
-  succMany?_add_one n x := by
-    rw [← ofBitVec_toBitVec x]
-    simp [succMany?_ofBitVec, succMany?_add_one, Option.bind_map, Function.comp_def,
-      succ?_ofBitVec, -ofBitVec_toBitVec]
-
-private theorem toBitVec_le {x y : Int16} :
-    x.toBitVec ≤ y.toBitVec ↔ x ≤ y := by
-  rw [Int16.le_iff_toBitVec_sle]
-  simp [LE.le]
-
-private theorem ofBitVec_le {x y : BitVec 16} :
-    Int16.ofBitVec x ≤ Int16.ofBitVec y ↔ x ≤ y := by
-  simp [← toBitVec_le]
-
-instance : LawfulUpwardEnumerableLE Int16 where
-  le_iff x y := by
-    rw [← ofBitVec_toBitVec x, ← ofBitVec_toBitVec y]
-    simpa [upwardEnumerableLE_ofBitVec, -ofBitVec_toBitVec, ofBitVec_le] using
-      LawfulUpwardEnumerableLE.le_iff (α := BitVec 16) _ _
-
-instance : LawfulUpwardEnumerableLT Int16 := inferInstance
-instance : LawfulUpwardEnumerableLT Int16 := inferInstance
-
-instance : Rxc.HasSize Int16 where
-  size lo hi := (hi.toInt + 1 - lo.toInt).toNat
-
-theorem rxcHasSize_eq_toBitVec :
-    Rxc.HasSize.size (Int16.ofBitVec lo) hi = Rxc.HasSize.size lo hi.toBitVec := by
-  simp [Rxc.HasSize.size, rotate, ← toInt_toBitVec, toInt_eq_ofNat_toNat_rotate_sub]
-  omega
-
-private theorem ofBitVec_eq_iff {x : BitVec 16} {y : Int16} :
-    Int16.ofBitVec x = y ↔ x = y.toBitVec := by
-  rw [← toBitVec_ofBitVec x, toBitVec_inj, toBitVec_ofBitVec]
-
-instance : Rxc.LawfulHasSize Int16 where
-  size_eq_zero_of_not_le lo hi := by
-    rw [← ofBitVec_toBitVec lo, ← ofBitVec_toBitVec hi]
-    simpa [rxcHasSize_eq_toBitVec, UInt16.lt_iff_toBitVec_lt, ofBitVec_le, -ofBitVec_toBitVec] using
-      Rxc.LawfulHasSize.size_eq_zero_of_not_le (α := BitVec 16) _ _
-  size_eq_one_of_succ?_eq_none lo hi := by
-    rw [← ofBitVec_toBitVec lo, ← ofBitVec_toBitVec hi]
-    simpa [rxcHasSize_eq_toBitVec, UInt16.le_iff_toBitVec_le, succ?_ofBitVec, ofBitVec_le,
-      -ofBitVec_toBitVec] using Rxc.LawfulHasSize.size_eq_one_of_succ?_eq_none (α := BitVec 16) _ _
-  size_eq_succ_of_succ?_eq_some lo hi x := by
-    rw [← ofBitVec_toBitVec lo, ← ofBitVec_toBitVec x, ← ofBitVec_toBitVec hi]
-    simpa [rxcHasSize_eq_toBitVec, UInt16.le_iff_toBitVec_le, ← UInt16.toBitVec_inj,
-      ofBitVec_le, succ?_ofBitVec, -ofBitVec_toBitVec, ofBitVec_eq_iff] using
-      Rxc.LawfulHasSize.size_eq_succ_of_succ?_eq_some (α := BitVec 16) _ _ _
-
-instance : Rxc.IsAlwaysFinite Int16 := inferInstance
-
-instance : Rxo.HasSize Int16 := .ofClosed
-instance : Rxo.LawfulHasSize Int16 := inferInstance
-instance : Rxo.IsAlwaysFinite Int16 := inferInstance
-
-instance : Rxi.HasSize Int16 where
-  size lo := ((2 : Int) ^ 15 - lo.toInt).toNat
-
-theorem rxiHasSize_eq_toBitVec :
-    Rxi.HasSize.size (Int16.ofBitVec lo) = Rxi.HasSize.size lo := by
-  simp [Rxi.HasSize.size, rotate, toInt_eq_ofNat_toNat_rotate_sub]
-  omega
-
-instance : Rxi.LawfulHasSize Int16 where
-  size_eq_one_of_succ?_eq_none lo := by
-    rw [← ofBitVec_toBitVec lo]
-    simpa [rxiHasSize_eq_toBitVec, succ?_ofBitVec, -ofBitVec_toBitVec] using
-      Rxi.LawfulHasSize.size_eq_one_of_succ?_eq_none (α := BitVec 16) _
-  size_eq_succ_of_succ?_eq_some lo lo' := by
-    rw [← ofBitVec_toBitVec lo, ← ofBitVec_toBitVec lo']
-    simpa [rxiHasSize_eq_toBitVec, succ?_ofBitVec, ofBitVec_eq_iff, -ofBitVec_toBitVec] using
-      Rxi.LawfulHasSize.size_eq_succ_of_succ?_eq_some (α := BitVec 16) _ _
-
-end Int16
-
 namespace Int32
 
 open BitVec.Signed
+open scoped HasModel
 
-attribute [-instance] BitVec.instUpwardEnumerable BitVec.instHasSize BitVec.instHasSize_1
-  BitVec.instHasSize_2 BitVec.instLawfulUpwardEnumerable
+@[inline] def irredMin := Int32.minValue
+@[inline] def irredMax := Int32.maxValue
+theorem irredMin_def : irredMin = Int32.minValue := (rfl)
+theorem irredMax_def : irredMax = Int32.maxValue := (rfl)
+seal irredMin irredMax
+
+theorem toBitVec_irredMin_eq_irredMin : irredMin.toBitVec = BitVec.Signed.irredMin 32 := by
+  simp [irredMin_def, BitVec.Signed.irredMin_def]
+theorem toBitVec_irredMax_eq_irredMax : irredMax.toBitVec = BitVec.Signed.irredMax 32 := by
+  simp [irredMax_def, BitVec.Signed.irredMax_def]
 
 instance : UpwardEnumerable Int32 where
-  succ? i := if i + 1 = Int32.minValue then none else some (i + 1)
+  succ? i := if i + 1 = irredMin then none else some (i + 1)
   succMany? n i :=
     have := i.minValue_le_toInt
-    if h : i.toInt + n ≤ Int32.maxValue.toInt then some (.ofIntLE _ (by omega) h) else none
+    if h : i.toInt + n ≤ irredMax.toInt then some (.ofIntLE _ (by omega) (irredMax_def ▸ h)) else none
 
-theorem succ?_ofBitVec {x : BitVec 32} :
-    UpwardEnumerable.succ? (Int32.ofBitVec x) = Int32.ofBitVec <$> UpwardEnumerable.succ? x := by
-  simp only [succ?, ← toBitVec_inj, Int32.toBitVec_add, toBitVec_ofBitVec, toBitVec_ofNat,
-    BitVec.ofNat_eq_ofNat, toBitVec_neg, BitVec.reduceNeg, rotate, BitVec.natCast_eq_ofNat,
-    Option.map_eq_map, Option.map_map, Function.comp_def]
-  split <;> split <;> try (simp_all [Int32.add_assoc]; done)
-  all_goals
-    rename_i h h'
-    rw [BitVec.add_assoc, BitVec.add_comm 2147483648#32 1#32, ← BitVec.add_assoc,
-      ← BitVec.eq_sub_iff_add_eq] at h'
-    simp [h] at h'
+instance : HasModel Int32 (BitVec 32) where
+  encode x := x.toBitVec
+  decode x := .ofBitVec x
+  encode_decode := by simp
+  decode_encode := by simp
+  le_iff_encode_le := by simp [Int32.le_iff_toBitVec_sle, BitVec.Signed.instLE]
+  lt_iff_encode_lt := by simp [Int32.lt_iff_toBitVec_slt, BitVec.Signed.instLT]
 
-theorem succMany?_ofBitVec {k : Nat} {x : BitVec 32} :
-    UpwardEnumerable.succMany? k (Int32.ofBitVec x) =
-      Int32.ofBitVec <$> UpwardEnumerable.succMany? k x := by
-  simp only [succMany?, maxValue, ofIntLE_eq_ofInt, ofInt_add, dite_eq_ite, rotate,
-    BitVec.ofNatLT_eq_ofNat, Option.map_eq_map, Option.map_if, ofBitVec_add, ofBitVec_ofNat,
-    ofNat_add, ofNat_bitVecToNat]
-  split <;> split <;> try (simp [← ofBitVec_ofInt, Int32.add_assoc, Int32.add_comm (-2147483648)]; done)
-  all_goals
-    rename_i h h'
-    simp [toInt_eq_ofNat_toNat_rotate_sub, rotate] at h h'
-    omega
+private theorem ofBitVec_eq_iff {x : BitVec 32} {y : Int32} :
+    Int32.ofBitVec x = y ↔ x = y.toBitVec := by
+  rw [← toBitVec_ofBitVec x, toBitVec_inj, toBitVec_ofBitVec]
 
-theorem upwardEnumerableLE_ofBitVec {x y : BitVec 32} :
-    UpwardEnumerable.LE (Int32.ofBitVec x) (Int32.ofBitVec y) ↔ UpwardEnumerable.LE x y := by
-  simp [UpwardEnumerable.LE, succMany?_ofBitVec, ofBitVec_inj]
+theorem instUpwardEnumerable_eq :
+    instUpwardEnumerable = HasModel.instUpwardEnumerable := by
+  apply UpwardEnumerable.ext
+  · apply funext; intro x
+    apply HasModel.general_succ?
+    simp [HasModel.encode, succ?, ← Int32.toBitVec_inj, toBitVec_irredMin_eq_irredMin]
+  · ext
+    simp [HasModel.general_succMany?, instUpwardEnumerable, HasModel.encode, HasModel.decode,
+      ← toInt_toBitVec, toBitVec_irredMax_eq_irredMax, ofIntLE_eq_ofInt]
 
-theorem upwardEnumerableLT_ofBitVec {x y : BitVec 32} :
-    UpwardEnumerable.LT (Int32.ofBitVec x) (Int32.ofBitVec y) ↔ UpwardEnumerable.LT x y := by
-  simp [UpwardEnumerable.LT, succMany?_ofBitVec, ofBitVec_inj]
+instance : LawfulUpwardEnumerable Int32 := by
+  simp only [instUpwardEnumerable_eq]
+  infer_instance
 
-instance : LawfulUpwardEnumerable Int32 where
-  ne_of_lt x y := by
-    rw [← ofBitVec_toBitVec x, ← ofBitVec_toBitVec y]
-    simpa [upwardEnumerableLT_ofBitVec, ne_iff_ofBitVec_ne, -ofBitVec_toBitVec] using
-      LawfulUpwardEnumerable.ne_of_lt (α := BitVec 32) _ _
-  succMany?_zero x := by
-    rw [← ofBitVec_toBitVec x]
-    simpa [succMany?_ofBitVec, ofBitVec_inj, -ofBitVec_toBitVec] using succMany?_zero
-  succMany?_add_one n x := by
-    rw [← ofBitVec_toBitVec x]
-    simp [succMany?_ofBitVec, succMany?_add_one, Option.bind_map, Function.comp_def,
-      succ?_ofBitVec, -ofBitVec_toBitVec]
-
-private theorem toBitVec_le {x y : Int32} :
-    x.toBitVec ≤ y.toBitVec ↔ x ≤ y := by
-  rw [Int32.le_iff_toBitVec_sle]
-  simp [LE.le]
-
-private theorem ofBitVec_le {x y : BitVec 32} :
-    Int32.ofBitVec x ≤ Int32.ofBitVec y ↔ x ≤ y := by
-  simp [← toBitVec_le]
-
-instance : LawfulUpwardEnumerableLE Int32 where
-  le_iff x y := by
-    rw [← ofBitVec_toBitVec x, ← ofBitVec_toBitVec y]
-    simpa [upwardEnumerableLE_ofBitVec, -ofBitVec_toBitVec, ofBitVec_le] using
-      LawfulUpwardEnumerableLE.le_iff (α := BitVec 32) _ _
+instance : LawfulUpwardEnumerableLE Int32 := by
+  simp only [instUpwardEnumerable_eq]
+  infer_instance
 
 instance : LawfulUpwardEnumerableLT Int32 := inferInstance
 instance : LawfulUpwardEnumerableLT Int32 := inferInstance
@@ -989,321 +428,211 @@ instance : LawfulUpwardEnumerableLT Int32 := inferInstance
 instance : Rxc.HasSize Int32 where
   size lo hi := (hi.toInt + 1 - lo.toInt).toNat
 
-def offset : BitVec 32 := 2 ^ 32 - 1
+theorem instRxcHasSize_eq :
+    instHasSize = HasModel.instRxcHasSize := by
+  simp only [instHasSize, HasModel.instRxcHasSize, Rxc.HasSize.size, HasModel.encode,
+    ← toInt_toBitVec, HasModel.general_rxcSize (Nat.zero_lt_succ _)]
 
-theorem bla {lo hi : BitVec n} (h : n > 0) :
-    (hi.toInt + 1 - lo.toInt).toNat = (rotate hi).toNat + 1 - (rotate lo).toNat := by
-  match n with
-  | 0 => omega
-  | n + 1 =>
-    simp only [toInt_eq_ofNat_toNat_rotate_sub h, rotate, BitVec.toNat_add, Int.natCast_emod,
-      show ∀ a b c d : Int, (a - b) + c - (d - b) = a + c - d by omega]
-    omega
-
-theorem rxcHasSize_eq_toBitVec :
-    Rxc.HasSize.size (Int32.ofBitVec lo) hi = Rxc.HasSize.size lo hi.toBitVec := by
-  rw [← ofBitVec_toBitVec (x := hi)]
-  generalize hi.toBitVec = hi
-  simp only [Rxc.HasSize.size, toInt_ofBitVec, toBitVec_ofBitVec]
-  apply bla
-
-private theorem ofBitVec_eq_iff {x : BitVec 32} {y : Int32} :
-    Int32.ofBitVec x = y ↔ x = y.toBitVec := by
-  rw [← toBitVec_ofBitVec x, toBitVec_inj, toBitVec_ofBitVec]
-
-instance : Rxc.LawfulHasSize Int32 where
-  size_eq_zero_of_not_le lo hi := by
-    rw [← ofBitVec_toBitVec lo, ← ofBitVec_toBitVec hi]
-    simpa [rxcHasSize_eq_toBitVec, UInt32.lt_iff_toBitVec_lt, ofBitVec_le, -ofBitVec_toBitVec] using
-      Rxc.LawfulHasSize.size_eq_zero_of_not_le (α := BitVec 32) _ _
-  size_eq_one_of_succ?_eq_none lo hi := by
-    rw [← ofBitVec_toBitVec lo, ← ofBitVec_toBitVec hi]
-    simpa [rxcHasSize_eq_toBitVec, UInt32.le_iff_toBitVec_le, succ?_ofBitVec, ofBitVec_le,
-      -ofBitVec_toBitVec] using Rxc.LawfulHasSize.size_eq_one_of_succ?_eq_none (α := BitVec 32) _ _
-  size_eq_succ_of_succ?_eq_some lo hi x := by
-    rw [← ofBitVec_toBitVec lo, ← ofBitVec_toBitVec x, ← ofBitVec_toBitVec hi]
-    simpa [rxcHasSize_eq_toBitVec, UInt32.le_iff_toBitVec_le, ← UInt32.toBitVec_inj,
-      ofBitVec_le, succ?_ofBitVec, -ofBitVec_toBitVec, ofBitVec_eq_iff] using
-      Rxc.LawfulHasSize.size_eq_succ_of_succ?_eq_some (α := BitVec 32) _ _ _
-
+instance : Rxc.LawfulHasSize Int32 := by
+  simp only [instUpwardEnumerable_eq, instRxcHasSize_eq]
+  infer_instance
 instance : Rxc.IsAlwaysFinite Int32 := inferInstance
 
 instance : Rxo.HasSize Int32 := .ofClosed
 instance : Rxo.LawfulHasSize Int32 := inferInstance
 instance : Rxo.IsAlwaysFinite Int32 := inferInstance
 
-instance : Rxi.HasSize Int32 where
+instance instRxiHasSize : Rxi.HasSize Int32 where
   size lo := ((2 : Int) ^ 31 - lo.toInt).toNat
 
-theorem rxiHasSize_eq_toBitVec :
-    Rxi.HasSize.size (Int32.ofBitVec lo) = Rxi.HasSize.size lo := by
-  simp [Rxi.HasSize.size, rotate, toInt_eq_ofNat_toNat_rotate_sub]
-  omega
+theorem instRxiHasSize_eq :
+    instRxiHasSize = HasModel.instRxiHasSize := by
+  simp only [instRxiHasSize, HasModel.instRxiHasSize, Rxi.HasSize.size, ← toInt_toBitVec,
+    HasModel.encode, HasModel.general_rxiSize (show 32 > 0 by omega)]
 
-instance : Rxi.LawfulHasSize Int32 where
-  size_eq_one_of_succ?_eq_none lo := by
-    rw [← ofBitVec_toBitVec lo]
-    simpa [rxiHasSize_eq_toBitVec, succ?_ofBitVec, -ofBitVec_toBitVec] using
-      Rxi.LawfulHasSize.size_eq_one_of_succ?_eq_none (α := BitVec 32) _
-  size_eq_succ_of_succ?_eq_some lo lo' := by
-    rw [← ofBitVec_toBitVec lo, ← ofBitVec_toBitVec lo']
-    simpa [rxiHasSize_eq_toBitVec, succ?_ofBitVec, ofBitVec_eq_iff, -ofBitVec_toBitVec] using
-      Rxi.LawfulHasSize.size_eq_succ_of_succ?_eq_some (α := BitVec 32) _ _
+instance : Rxi.LawfulHasSize Int32 := by
+  simp only [instUpwardEnumerable_eq, instRxiHasSize_eq]
+  infer_instance
+instance : Rxi.IsAlwaysFinite Int32 := inferInstance
 
 end Int32
-namespace Int8
+
+namespace Int64
 
 open BitVec.Signed
+open scoped HasModel
 
-attribute [-instance] BitVec.instUpwardEnumerable BitVec.instHasSize BitVec.instHasSize_1
-  BitVec.instHasSize_2 BitVec.instLawfulUpwardEnumerable
+@[inline] def irredMin := Int64.minValue
+@[inline] def irredMax := Int64.maxValue
+theorem irredMin_def : irredMin = Int64.minValue := (rfl)
+theorem irredMax_def : irredMax = Int64.maxValue := (rfl)
+seal irredMin irredMax
 
-instance : UpwardEnumerable Int8 where
-  succ? i := if i + 1 = Int8.minValue then none else some (i + 1)
+theorem toBitVec_irredMin_eq_irredMin : irredMin.toBitVec = BitVec.Signed.irredMin 64 := by
+  simp [irredMin_def, BitVec.Signed.irredMin_def]
+theorem toBitVec_irredMax_eq_irredMax : irredMax.toBitVec = BitVec.Signed.irredMax 64 := by
+  simp [irredMax_def, BitVec.Signed.irredMax_def]
+
+instance : UpwardEnumerable Int64 where
+  succ? i := if i + 1 = irredMin then none else some (i + 1)
   succMany? n i :=
     have := i.minValue_le_toInt
-    if h : i.toInt + n ≤ Int8.maxValue.toInt then some (.ofIntLE _ (by omega) h) else none
+    if h : i.toInt + n ≤ irredMax.toInt then some (.ofIntLE _ (by omega) (irredMax_def ▸ h)) else none
 
-theorem succ?_ofBitVec {x : BitVec 8} :
-    UpwardEnumerable.succ? (Int8.ofBitVec x) = Int8.ofBitVec <$> UpwardEnumerable.succ? x := by
-  simp only [succ?, ← toBitVec_inj, Int8.toBitVec_add, toBitVec_ofBitVec, toBitVec_ofNat,
-    BitVec.ofNat_eq_ofNat, toBitVec_neg, BitVec.reduceNeg, rotate, BitVec.natCast_eq_ofNat,
-    Option.map_eq_map, Option.map_map, Function.comp_def]
-  split <;> split <;> try (simp_all [Int8.add_assoc]; done)
-  all_goals
-    rename_i h h'
-    rw [BitVec.add_assoc, BitVec.add_comm 128#8 1#8, ← BitVec.add_assoc,
-      ← BitVec.eq_sub_iff_add_eq] at h'
-    simp [h] at h'
+instance : HasModel Int64 (BitVec 64) where
+  encode x := x.toBitVec
+  decode x := .ofBitVec x
+  encode_decode := by simp
+  decode_encode := by simp
+  le_iff_encode_le := by simp [Int64.le_iff_toBitVec_sle, BitVec.Signed.instLE]
+  lt_iff_encode_lt := by simp [Int64.lt_iff_toBitVec_slt, BitVec.Signed.instLT]
 
-theorem succMany?_ofBitVec {k : Nat} {x : BitVec 8} :
-    UpwardEnumerable.succMany? k (Int8.ofBitVec x) =
-      Int8.ofBitVec <$> UpwardEnumerable.succMany? k x := by
-  simp only [succMany?, maxValue, ofIntLE_eq_ofInt, ofInt_add, dite_eq_ite, rotate,
-    BitVec.ofNatLT_eq_ofNat, Option.map_eq_map, Option.map_if, ofBitVec_add, ofBitVec_ofNat,
-    ofNat_add, ofNat_bitVecToNat]
-  split <;> split <;> try (simp [← ofBitVec_ofInt, Int8.add_assoc, Int8.add_comm (-128)]; done)
-  all_goals
-    rename_i h h'
-    simp [toInt_eq_ofNat_toNat_rotate_sub, rotate] at h h'
-    omega
-
-theorem upwardEnumerableLE_ofBitVec {x y : BitVec 8} :
-    UpwardEnumerable.LE (Int8.ofBitVec x) (Int8.ofBitVec y) ↔ UpwardEnumerable.LE x y := by
-  simp [UpwardEnumerable.LE, succMany?_ofBitVec, ofBitVec_inj]
-
-theorem upwardEnumerableLT_ofBitVec {x y : BitVec 8} :
-    UpwardEnumerable.LT (Int8.ofBitVec x) (Int8.ofBitVec y) ↔ UpwardEnumerable.LT x y := by
-  simp [UpwardEnumerable.LT, succMany?_ofBitVec, ofBitVec_inj]
-
-instance : LawfulUpwardEnumerable Int8 where
-  ne_of_lt x y := by
-    rw [← ofBitVec_toBitVec x, ← ofBitVec_toBitVec y]
-    simpa [upwardEnumerableLT_ofBitVec, ne_iff_ofBitVec_ne, -ofBitVec_toBitVec] using
-      LawfulUpwardEnumerable.ne_of_lt (α := BitVec 8) _ _
-  succMany?_zero x := by
-    rw [← ofBitVec_toBitVec x]
-    simpa [succMany?_ofBitVec, ofBitVec_inj, -ofBitVec_toBitVec] using succMany?_zero
-  succMany?_add_one n x := by
-    rw [← ofBitVec_toBitVec x]
-    simp [succMany?_ofBitVec, succMany?_add_one, Option.bind_map, Function.comp_def,
-      succ?_ofBitVec, -ofBitVec_toBitVec]
-
-private theorem toBitVec_le {x y : Int8} :
-    x.toBitVec ≤ y.toBitVec ↔ x ≤ y := by
-  rw [Int8.le_iff_toBitVec_sle]
-  simp [LE.le]
-
-private theorem ofBitVec_le {x y : BitVec 8} :
-    Int8.ofBitVec x ≤ Int8.ofBitVec y ↔ x ≤ y := by
-  simp [← toBitVec_le]
-
-instance : LawfulUpwardEnumerableLE Int8 where
-  le_iff x y := by
-    rw [← ofBitVec_toBitVec x, ← ofBitVec_toBitVec y]
-    simpa [upwardEnumerableLE_ofBitVec, -ofBitVec_toBitVec, ofBitVec_le] using
-      LawfulUpwardEnumerableLE.le_iff (α := BitVec 8) _ _
-
-instance : LawfulUpwardEnumerableLT Int8 := inferInstance
-instance : LawfulUpwardEnumerableLT Int8 := inferInstance
-
-instance : Rxc.HasSize Int8 where
-  size lo hi := (hi.toInt + 1 - lo.toInt).toNat
-
-theorem rxcHasSize_eq_toBitVec :
-    Rxc.HasSize.size (Int8.ofBitVec lo) hi = Rxc.HasSize.size lo hi.toBitVec := by
-  simp [Rxc.HasSize.size, rotate, ← toInt_toBitVec, toInt_eq_ofNat_toNat_rotate_sub]
-  omega
-
-private theorem ofBitVec_eq_iff {x : BitVec 8} {y : Int8} :
-    Int8.ofBitVec x = y ↔ x = y.toBitVec := by
+private theorem ofBitVec_eq_iff {x : BitVec 64} {y : Int64} :
+    Int64.ofBitVec x = y ↔ x = y.toBitVec := by
   rw [← toBitVec_ofBitVec x, toBitVec_inj, toBitVec_ofBitVec]
 
-instance : Rxc.LawfulHasSize Int8 where
-  size_eq_zero_of_not_le lo hi := by
-    rw [← ofBitVec_toBitVec lo, ← ofBitVec_toBitVec hi]
-    simpa [rxcHasSize_eq_toBitVec, UInt8.lt_iff_toBitVec_lt, ofBitVec_le, -ofBitVec_toBitVec] using
-      Rxc.LawfulHasSize.size_eq_zero_of_not_le (α := BitVec 8) _ _
-  size_eq_one_of_succ?_eq_none lo hi := by
-    rw [← ofBitVec_toBitVec lo, ← ofBitVec_toBitVec hi]
-    simpa [rxcHasSize_eq_toBitVec, UInt8.le_iff_toBitVec_le, succ?_ofBitVec, ofBitVec_le,
-      -ofBitVec_toBitVec] using Rxc.LawfulHasSize.size_eq_one_of_succ?_eq_none (α := BitVec 8) _ _
-  size_eq_succ_of_succ?_eq_some lo hi x := by
-    rw [← ofBitVec_toBitVec lo, ← ofBitVec_toBitVec x, ← ofBitVec_toBitVec hi]
-    simpa [rxcHasSize_eq_toBitVec, UInt8.le_iff_toBitVec_le, ← UInt8.toBitVec_inj,
-      ofBitVec_le, succ?_ofBitVec, -ofBitVec_toBitVec, ofBitVec_eq_iff] using
-      Rxc.LawfulHasSize.size_eq_succ_of_succ?_eq_some (α := BitVec 8) _ _ _
+theorem instUpwardEnumerable_eq :
+    instUpwardEnumerable = HasModel.instUpwardEnumerable := by
+  apply UpwardEnumerable.ext
+  · apply funext; intro x
+    apply HasModel.general_succ?
+    simp [HasModel.encode, succ?, ← Int64.toBitVec_inj, toBitVec_irredMin_eq_irredMin]
+  · ext
+    simp [HasModel.general_succMany?, instUpwardEnumerable, HasModel.encode, HasModel.decode,
+      ← toInt_toBitVec, toBitVec_irredMax_eq_irredMax, ofIntLE_eq_ofInt]
 
-instance : Rxc.IsAlwaysFinite Int8 := inferInstance
+instance : LawfulUpwardEnumerable Int64 := by
+  simp only [instUpwardEnumerable_eq]
+  infer_instance
 
-instance : Rxo.HasSize Int8 := .ofClosed
-instance : Rxo.LawfulHasSize Int8 := inferInstance
-instance : Rxo.IsAlwaysFinite Int8 := inferInstance
+instance : LawfulUpwardEnumerableLE Int64 := by
+  simp only [instUpwardEnumerable_eq]
+  infer_instance
 
-instance : Rxi.HasSize Int8 where
-  size lo := ((2 : Int) ^ 7 - lo.toInt).toNat
+instance : LawfulUpwardEnumerableLT Int64 := inferInstance
+instance : LawfulUpwardEnumerableLT Int64 := inferInstance
 
-theorem rxiHasSize_eq_toBitVec :
-    Rxi.HasSize.size (Int8.ofBitVec lo) = Rxi.HasSize.size lo := by
-  simp [Rxi.HasSize.size, rotate, toInt_eq_ofNat_toNat_rotate_sub]
-  omega
+instance : Rxc.HasSize Int64 where
+  size lo hi := (hi.toInt + 1 - lo.toInt).toNat
 
-instance : Rxi.LawfulHasSize Int8 where
-  size_eq_one_of_succ?_eq_none lo := by
-    rw [← ofBitVec_toBitVec lo]
-    simpa [rxiHasSize_eq_toBitVec, succ?_ofBitVec, -ofBitVec_toBitVec] using
-      Rxi.LawfulHasSize.size_eq_one_of_succ?_eq_none (α := BitVec 8) _
-  size_eq_succ_of_succ?_eq_some lo lo' := by
-    rw [← ofBitVec_toBitVec lo, ← ofBitVec_toBitVec lo']
-    simpa [rxiHasSize_eq_toBitVec, succ?_ofBitVec, ofBitVec_eq_iff, -ofBitVec_toBitVec] using
-      Rxi.LawfulHasSize.size_eq_succ_of_succ?_eq_some (α := BitVec 8) _ _
+theorem instRxcHasSize_eq :
+    instHasSize = HasModel.instRxcHasSize := by
+  simp only [instHasSize, HasModel.instRxcHasSize, Rxc.HasSize.size, HasModel.encode,
+    ← toInt_toBitVec, HasModel.general_rxcSize (Nat.zero_lt_succ _)]
 
-end Int8
-namespace Int8
+instance : Rxc.LawfulHasSize Int64 := by
+  simp only [instUpwardEnumerable_eq, instRxcHasSize_eq]
+  infer_instance
+instance : Rxc.IsAlwaysFinite Int64 := inferInstance
+
+instance : Rxo.HasSize Int64 := .ofClosed
+instance : Rxo.LawfulHasSize Int64 := inferInstance
+instance : Rxo.IsAlwaysFinite Int64 := inferInstance
+
+instance instRxiHasSize : Rxi.HasSize Int64 where
+  size lo := ((2 : Int) ^ 63 - lo.toInt).toNat
+
+theorem instRxiHasSize_eq :
+    instRxiHasSize = HasModel.instRxiHasSize := by
+  simp only [instRxiHasSize, HasModel.instRxiHasSize, Rxi.HasSize.size, ← toInt_toBitVec,
+    HasModel.encode, HasModel.general_rxiSize (show 64 > 0 by omega)]
+
+instance : Rxi.LawfulHasSize Int64 := by
+  simp only [instUpwardEnumerable_eq, instRxiHasSize_eq]
+  infer_instance
+instance : Rxi.IsAlwaysFinite Int64 := inferInstance
+
+end Int64
+
+namespace ISize
 
 open BitVec.Signed
+open scoped HasModel
 
-attribute [-instance] BitVec.instUpwardEnumerable BitVec.instHasSize BitVec.instHasSize_1
-  BitVec.instHasSize_2 BitVec.instLawfulUpwardEnumerable
+@[inline] def irredMin := ISize.minValue
+@[inline] def irredMax := ISize.maxValue
+theorem irredMin_def : irredMin = ISize.minValue := (rfl)
+theorem irredMax_def : irredMax = ISize.maxValue := (rfl)
+seal irredMin irredMax
 
-instance : UpwardEnumerable Int8 where
-  succ? i := if i + 1 = Int8.minValue then none else some (i + 1)
+theorem toBitVec_irredMin_eq_irredMin :
+    irredMin.toBitVec = BitVec.Signed.irredMin System.Platform.numBits := by
+  rw [irredMin_def, BitVec.Signed.irredMin_def, toBitVec_minValue]
+  have := System.Platform.numBits_eq; generalize System.Platform.numBits = a at this ⊢
+  rcases this with rfl | rfl <;> rfl
+theorem toBitVec_irredMax_eq_irredMax :
+    irredMax.toBitVec = BitVec.Signed.irredMax System.Platform.numBits := by
+  rw [irredMax_def, BitVec.Signed.irredMax_def, toBitVec_maxValue]
+  have := System.Platform.numBits_eq; generalize System.Platform.numBits = a at this ⊢
+  rcases this with rfl | rfl <;> rfl
+
+instance : UpwardEnumerable ISize where
+  succ? i := if i + 1 = irredMin then none else some (i + 1)
   succMany? n i :=
     have := i.minValue_le_toInt
-    if h : i.toInt + n ≤ Int8.maxValue.toInt then some (.ofIntLE _ (by omega) h) else none
+    if h : i.toInt + n ≤ irredMax.toInt then some (.ofIntLE _ (by omega) (irredMax_def ▸ h)) else none
 
-theorem succ?_ofBitVec {x : BitVec 8} :
-    UpwardEnumerable.succ? (Int8.ofBitVec x) = Int8.ofBitVec <$> UpwardEnumerable.succ? x := by
-  simp only [succ?, ← toBitVec_inj, Int8.toBitVec_add, toBitVec_ofBitVec, toBitVec_ofNat,
-    BitVec.ofNat_eq_ofNat, toBitVec_neg, BitVec.reduceNeg, rotate, BitVec.natCast_eq_ofNat,
-    Option.map_eq_map, Option.map_map, Function.comp_def]
-  split <;> split <;> try (simp_all [Int8.add_assoc]; done)
-  all_goals
-    rename_i h h'
-    rw [BitVec.add_assoc, BitVec.add_comm 128#8 1#8, ← BitVec.add_assoc,
-      ← BitVec.eq_sub_iff_add_eq] at h'
-    simp [h] at h'
+instance : HasModel ISize (BitVec System.Platform.numBits) where
+  encode x := x.toBitVec
+  decode x := .ofBitVec x
+  encode_decode := by simp
+  decode_encode := by simp
+  le_iff_encode_le := by simp [ISize.le_iff_toBitVec_sle, BitVec.Signed.instLE]
+  lt_iff_encode_lt := by simp [ISize.lt_iff_toBitVec_slt, BitVec.Signed.instLT]
 
-theorem succMany?_ofBitVec {k : Nat} {x : BitVec 8} :
-    UpwardEnumerable.succMany? k (Int8.ofBitVec x) =
-      Int8.ofBitVec <$> UpwardEnumerable.succMany? k x := by
-  simp only [succMany?, maxValue, ofIntLE_eq_ofInt, ofInt_add, dite_eq_ite, rotate,
-    BitVec.ofNatLT_eq_ofNat, Option.map_eq_map, Option.map_if, ofBitVec_add, ofBitVec_ofNat,
-    ofNat_add, ofNat_bitVecToNat]
-  split <;> split <;> try (simp [← ofBitVec_ofInt, Int8.add_assoc, Int8.add_comm (-128)]; done)
-  all_goals
-    rename_i h h'
-    simp [toInt_eq_ofNat_toNat_rotate_sub, rotate] at h h'
-    omega
-
-theorem upwardEnumerableLE_ofBitVec {x y : BitVec 8} :
-    UpwardEnumerable.LE (Int8.ofBitVec x) (Int8.ofBitVec y) ↔ UpwardEnumerable.LE x y := by
-  simp [UpwardEnumerable.LE, succMany?_ofBitVec, ofBitVec_inj]
-
-theorem upwardEnumerableLT_ofBitVec {x y : BitVec 8} :
-    UpwardEnumerable.LT (Int8.ofBitVec x) (Int8.ofBitVec y) ↔ UpwardEnumerable.LT x y := by
-  simp [UpwardEnumerable.LT, succMany?_ofBitVec, ofBitVec_inj]
-
-instance : LawfulUpwardEnumerable Int8 where
-  ne_of_lt x y := by
-    rw [← ofBitVec_toBitVec x, ← ofBitVec_toBitVec y]
-    simpa [upwardEnumerableLT_ofBitVec, ne_iff_ofBitVec_ne, -ofBitVec_toBitVec] using
-      LawfulUpwardEnumerable.ne_of_lt (α := BitVec 8) _ _
-  succMany?_zero x := by
-    rw [← ofBitVec_toBitVec x]
-    simpa [succMany?_ofBitVec, ofBitVec_inj, -ofBitVec_toBitVec] using succMany?_zero
-  succMany?_add_one n x := by
-    rw [← ofBitVec_toBitVec x]
-    simp [succMany?_ofBitVec, succMany?_add_one, Option.bind_map, Function.comp_def,
-      succ?_ofBitVec, -ofBitVec_toBitVec]
-
-private theorem toBitVec_le {x y : Int8} :
-    x.toBitVec ≤ y.toBitVec ↔ x ≤ y := by
-  rw [Int8.le_iff_toBitVec_sle]
-  simp [LE.le]
-
-private theorem ofBitVec_le {x y : BitVec 8} :
-    Int8.ofBitVec x ≤ Int8.ofBitVec y ↔ x ≤ y := by
-  simp [← toBitVec_le]
-
-instance : LawfulUpwardEnumerableLE Int8 where
-  le_iff x y := by
-    rw [← ofBitVec_toBitVec x, ← ofBitVec_toBitVec y]
-    simpa [upwardEnumerableLE_ofBitVec, -ofBitVec_toBitVec, ofBitVec_le] using
-      LawfulUpwardEnumerableLE.le_iff (α := BitVec 8) _ _
-
-instance : LawfulUpwardEnumerableLT Int8 := inferInstance
-instance : LawfulUpwardEnumerableLT Int8 := inferInstance
-
-instance : Rxc.HasSize Int8 where
-  size lo hi := (hi.toInt + 1 - lo.toInt).toNat
-
-theorem rxcHasSize_eq_toBitVec :
-    Rxc.HasSize.size (Int8.ofBitVec lo) hi = Rxc.HasSize.size lo hi.toBitVec := by
-  simp [Rxc.HasSize.size, rotate, ← toInt_toBitVec, toInt_eq_ofNat_toNat_rotate_sub]
-  omega
-
-private theorem ofBitVec_eq_iff {x : BitVec 8} {y : Int8} :
-    Int8.ofBitVec x = y ↔ x = y.toBitVec := by
+private theorem ofBitVec_eq_iff {x : BitVec System.Platform.numBits} {y : ISize} :
+    ISize.ofBitVec x = y ↔ x = y.toBitVec := by
   rw [← toBitVec_ofBitVec x, toBitVec_inj, toBitVec_ofBitVec]
 
-instance : Rxc.LawfulHasSize Int8 where
-  size_eq_zero_of_not_le lo hi := by
-    rw [← ofBitVec_toBitVec lo, ← ofBitVec_toBitVec hi]
-    simpa [rxcHasSize_eq_toBitVec, UInt8.lt_iff_toBitVec_lt, ofBitVec_le, -ofBitVec_toBitVec] using
-      Rxc.LawfulHasSize.size_eq_zero_of_not_le (α := BitVec 8) _ _
-  size_eq_one_of_succ?_eq_none lo hi := by
-    rw [← ofBitVec_toBitVec lo, ← ofBitVec_toBitVec hi]
-    simpa [rxcHasSize_eq_toBitVec, UInt8.le_iff_toBitVec_le, succ?_ofBitVec, ofBitVec_le,
-      -ofBitVec_toBitVec] using Rxc.LawfulHasSize.size_eq_one_of_succ?_eq_none (α := BitVec 8) _ _
-  size_eq_succ_of_succ?_eq_some lo hi x := by
-    rw [← ofBitVec_toBitVec lo, ← ofBitVec_toBitVec x, ← ofBitVec_toBitVec hi]
-    simpa [rxcHasSize_eq_toBitVec, UInt8.le_iff_toBitVec_le, ← UInt8.toBitVec_inj,
-      ofBitVec_le, succ?_ofBitVec, -ofBitVec_toBitVec, ofBitVec_eq_iff] using
-      Rxc.LawfulHasSize.size_eq_succ_of_succ?_eq_some (α := BitVec 8) _ _ _
+theorem instUpwardEnumerable_eq :
+    instUpwardEnumerable = HasModel.instUpwardEnumerable := by
+  apply UpwardEnumerable.ext
+  · apply funext; intro x
+    apply HasModel.general_succ?
+    simp [HasModel.encode, succ?, ← ISize.toBitVec_inj, toBitVec_irredMin_eq_irredMin]
+  · ext
+    simp [HasModel.general_succMany?, instUpwardEnumerable, HasModel.encode, HasModel.decode,
+      ← toInt_toBitVec, toBitVec_irredMax_eq_irredMax, ofIntLE_eq_ofInt]
 
-instance : Rxc.IsAlwaysFinite Int8 := inferInstance
+instance : LawfulUpwardEnumerable ISize := by
+  simp only [instUpwardEnumerable_eq]
+  infer_instance
 
-instance : Rxo.HasSize Int8 := .ofClosed
-instance : Rxo.LawfulHasSize Int8 := inferInstance
-instance : Rxo.IsAlwaysFinite Int8 := inferInstance
+instance : LawfulUpwardEnumerableLE ISize := by
+  simp only [instUpwardEnumerable_eq]
+  infer_instance
 
-instance : Rxi.HasSize Int8 where
-  size lo := ((2 : Int) ^ 7 - lo.toInt).toNat
+instance : LawfulUpwardEnumerableLT ISize := inferInstance
+instance : LawfulUpwardEnumerableLT ISize := inferInstance
 
-theorem rxiHasSize_eq_toBitVec :
-    Rxi.HasSize.size (Int8.ofBitVec lo) = Rxi.HasSize.size lo := by
-  simp [Rxi.HasSize.size, rotate, toInt_eq_ofNat_toNat_rotate_sub]
-  omega
+instance : Rxc.HasSize ISize where
+  size lo hi := (hi.toInt + 1 - lo.toInt).toNat
 
-instance : Rxi.LawfulHasSize Int8 where
-  size_eq_one_of_succ?_eq_none lo := by
-    rw [← ofBitVec_toBitVec lo]
-    simpa [rxiHasSize_eq_toBitVec, succ?_ofBitVec, -ofBitVec_toBitVec] using
-      Rxi.LawfulHasSize.size_eq_one_of_succ?_eq_none (α := BitVec 8) _
-  size_eq_succ_of_succ?_eq_some lo lo' := by
-    rw [← ofBitVec_toBitVec lo, ← ofBitVec_toBitVec lo']
-    simpa [rxiHasSize_eq_toBitVec, succ?_ofBitVec, ofBitVec_eq_iff, -ofBitVec_toBitVec] using
-      Rxi.LawfulHasSize.size_eq_succ_of_succ?_eq_some (α := BitVec 8) _ _
+theorem instRxcHasSize_eq :
+    instHasSize = HasModel.instRxcHasSize := by
+  simp only [instHasSize, HasModel.instRxcHasSize, Rxc.HasSize.size, HasModel.encode,
+    ← toInt_toBitVec, HasModel.general_rxcSize System.Platform.numBits_pos]
 
-end Int8
+instance : Rxc.LawfulHasSize ISize := by
+  simp only [instUpwardEnumerable_eq, instRxcHasSize_eq]
+  infer_instance
+instance : Rxc.IsAlwaysFinite ISize := inferInstance
+
+instance : Rxo.HasSize ISize := .ofClosed
+instance : Rxo.LawfulHasSize ISize := inferInstance
+instance : Rxo.IsAlwaysFinite ISize := inferInstance
+
+instance instRxiHasSize : Rxi.HasSize ISize where
+  size lo := ((2 : Int) ^ (System.Platform.numBits - 1) - lo.toInt).toNat
+
+theorem instRxiHasSize_eq :
+    instRxiHasSize = HasModel.instRxiHasSize := by
+  simp only [instRxiHasSize, HasModel.instRxiHasSize, Rxi.HasSize.size, ← toInt_toBitVec,
+    HasModel.encode, HasModel.general_rxiSize System.Platform.numBits_pos]
+
+instance : Rxi.LawfulHasSize ISize := by
+  simp only [instUpwardEnumerable_eq, instRxiHasSize_eq]
+  infer_instance
+instance : Rxi.IsAlwaysFinite ISize := inferInstance
+
+end ISize
